lib/sequences.dfy
@@ -8,7 +8,7 @@ module Sequences {
   function method DropLast<E>(run: seq<E>) : seq<E>
     requires |run| > 0;
   {
-	run[..|run|-1]
+    run[..|run|-1]
   }
 
   function method Set<T>(run: seq<T>) : set<T> {
